feat: inductive predicates

Test/Basic.lean
@@ -30,3 +30,39 @@ n m : Nat
 -/
 #guard_msgs in
 example (n m : Nat) : n.add m = m.add n := by nunchaku (timeout := 1)
+
+
+inductive MyEven : Nat → Prop where
+  | zero : MyEven Nat.zero
+  | succ : MyEven n → MyEven n.succ.succ
+
+/--
+info: The prover found a counter example
+---
+error: unsolved goals
+n : Nat
+⊢ MyEven n
+-/
+#guard_msgs in
+example (n : Nat) : MyEven n := by nunchaku
+
+/--
+info: The prover found a counter example
+---
+error: unsolved goals
+n : Nat
+h : MyEven n
+⊢ MyEven n.succ
+-/
+#guard_msgs in
+example (n : Nat) (h : MyEven n) : MyEven n.succ := by nunchaku
+
+/--
+info: The prover is convinced that the theorem is true.
+---
+error: unsolved goals
+n : Nat
+⊢ n ≠ n.succ
+-/
+#guard_msgs in
+example (n : Nat) : n ≠ n.succ := by nunchaku
